theories/quoteRecord.v
@@ -1,14 +1,17 @@
-From Coq Require Import List Strings.String ssreflect.
+From Coq Require Import List ssreflect.
 From MetaCoq.Template Require Import All.
 From Genxs Require Import metacoq_utils genDiscriminators.
 
 Set Primitive Projections.
 
-Import MonadNotation.
+Import MCMonadNotation.
 Import ListNotations.
 
 
-Run TemplateProgram (gen_discriminators false "option").
+(** Old WIP, I think the goal of this file was to generate the kind of functions found in unbundling.v *)
+
+
+MetaCoq Run (gen_discriminators false "option"%bs).
 (* Is there any way to manage implicit arguments from MetaCoq ? *)
 Arguments isSome {_} _.
 Arguments isNone {_} _.
@@ -19,9 +22,9 @@ Definition over_oien (oien : one_inductive_entry) (projs:list ident)
   match mind_entry_lc oien with
   |  (cty :: nil)%list =>
     let '(argnames, argtys, res)  := decompose_prod cty in
-    let filter '(name, _) :=
-      if name is nNamed id
-      then isNone (List.find (ident_eq id) projs)
+    let filter '(aname, _) :=
+      if aname.(binder_name) is nNamed id
+      then isNone (List.find (String.eqb id) projs)
       else true
     in
     let cty :=
@@ -30,45 +33,46 @@ Definition over_oien (oien : one_inductive_entry) (projs:list ident)
                         (List.filter filter
                                      (List.combine argnames argtys))
     in
-    let suffix := "_over_" ++ concat "_" projs in
+    let suffix := ("_over_" ++ String.concat "_" projs)%bs in
     ret (Build_one_inductive_entry
-           (mind_entry_typename oien ++ suffix)
+           (mind_entry_typename oien ++ suffix)%bs
            (mind_entry_arity oien)
-           (mind_entry_template oien)
-           (List.map (fun id => id ++ suffix) (mind_entry_consnames oien))
+           (List.map (fun id => id ++ suffix)%bs (mind_entry_consnames oien))
            (cty :: nil)%list)
-  | _ => tmFail "Not a record"
+  | _ => tmFail "Not a record"%bs
   end.
 
 Definition over_mien (mien:mutual_inductive_entry) (projs:list ident)
   : TemplateMonad mutual_inductive_entry :=
   id <- (match mind_entry_record mien with
         | Some (Some id) => ret id
-        | _ => tmFail "Not a record with primitive projection"
+        | _ => tmFail "Not a record with primitive projection"%bs
         end) ;;
   oien <- (match mind_entry_inds mien with
            | (oien :: nil)%list => ret oien
-           | _ => tmFail "Something is wrong over the internet"
+           | _ => tmFail "Something is wrong over the internet"%bs
            end) ;;
   oien <- over_oien oien projs ;;
-  let suffix := "_over_" ++ concat "_" projs in
+  let suffix := ("_over_" ++ String.concat "_" projs)%bs in
   ret (Build_mutual_inductive_entry
-         (Some (Some (id ++ suffix)))
+         (Some (Some (id ++ suffix)%bs))
          (mind_entry_finite mien)
          (mind_entry_params mien)
          (oien :: nil)%list
          (mind_entry_universes mien)
+         (mind_entry_template mien)
+         (mind_entry_variance mien)
          (mind_entry_private mien)).
-
-
 
 Definition mem {A} (eq:A -> A -> bool) (a:A) (l:list A) : bool := isSome (List.find (eq a) l).
 
+(*
 Definition over_oib (decl:mutual_inductive_body) (projs:list ident) (oid:one_inductive_body) :=
-  let suffix := "_over_" ++ concat "_" projs in
-  let filtered_projs := List.filter (fun '(id,_) => negb (mem ident_eq id projs)) (ind_projs oid) in
+  let suffix := ("_over_" ++ String.concat "_" projs)%bs in
+  let filtered_projs := List.filter (fun pb => negb (mem String.eqb pb.(proj_name) projs)) (ind_projs oid) in
   Build_one_inductive_body
-    (ind_name oid ++ suffix)
+    (ind_name oid ++ suffix)%bs
+    []%list
     (ind_type oid)
     (ind_kelim oid)
     (ind_ctors oid)
@@ -99,7 +103,7 @@ Module test.
       tmPrint t (* ;; *)
       (* tmMkInductive t_over_Ry *).
 
-  Run TemplateProgram prog.
+  MetaCoq Run prog.
 
   Definition prog2 : TemplateMonad unit :=
     t <- tmQuoteInductive "R";;
@@ -108,9 +112,9 @@ Module test.
       tmPrint t (* ;; *)
       (* tmMkInductive t_over_Ry *).
 
-  Run TemplateProgram prog2.
+  MetaCoq Run prog2.
 
-  (* Run TemplateProgram ( *)
+  (* MetaCoq Run ( *)
   (*   t <- tmQuoteInductive "R";; *)
   (*     t <- tmEval all (mind_body_to_entry t) ;; *)
   (*     tmMkInductive t;; *)
@@ -127,13 +131,15 @@ Axiom B : A -> Type.
 Axiom C : forall a, B a -> Type.
 
 Record T := mkT { t_a : A ; t_b : B t_a ; t_c : C _ t_b }.
-(* Run TemplateProgram (t <- tmQuoteInductive "T";; tmPrint t). *)
-(* Run TemplateProgram (x <- tmQuoteInductive "Top.T";; tmPrint x). *)
+(* MetaCoq Run (t <- tmQuoteInductive "T";; tmPrint t). *)
+(* MetaCoq Run (x <- tmQuoteInductive "Top.T";; tmPrint x). *)
 
 
-Run TemplateProgram (gen_discriminators false "recursivity_kind").
+MetaCoq Run (gen_discriminators false "recursivity_kind").
 
 
 (* Definition decomposeRecord (mindbody : mutual_inductive_body) *)
 (*   : TemplateMonad unit := *)
 (*   assertTM (isBiFinite (ind_finite mindbody)) ;; *)
+
+*)
